Rename some prod -> pair, sum -> either

src/defs/statics.lean
@@ -26,34 +26,34 @@ inductive has_typ: cx typ -> exp -> typ -> Prop
     has_typ Γ e2 τ1 ->
     has_typ Γ (exp.app e1 e2) τ2
 | unit {Γ: cx typ}: has_typ Γ exp.unit typ.unit
-| prod
+| pair
     {Γ: cx typ} {e1 e2: exp} {τ1 τ2: typ}:
     has_typ Γ e1 τ1 ->
     has_typ Γ e2 τ2 ->
-    has_typ Γ (exp.prod e1 e2) (typ.prod τ1 τ2)
-| prod_left
+    has_typ Γ (exp.pair e1 e2) (typ.pair τ1 τ2)
+| pair_left
     {Γ: cx typ} {e: exp} {τ1 τ2: typ}:
-    has_typ Γ e (typ.prod τ1 τ2) ->
-    has_typ Γ (exp.prod_left e) τ1
-| prod_right
+    has_typ Γ e (typ.pair τ1 τ2) ->
+    has_typ Γ (exp.pair_left e) τ1
+| pair_right
     {Γ: cx typ} {e: exp} {τ1 τ2: typ}:
-    has_typ Γ e (typ.prod τ1 τ2) ->
-    has_typ Γ (exp.prod_right e) τ2
-| sum_left
+    has_typ Γ e (typ.pair τ1 τ2) ->
+    has_typ Γ (exp.pair_right e) τ2
+| either_left
     {Γ: cx typ} {e: exp} {τ1 τ2: typ}:
     has_typ Γ e τ1 ->
-    has_typ Γ (exp.sum_left τ2 e) (typ.sum τ1 τ2)
-| sum_right
+    has_typ Γ (exp.either_left τ2 e) (typ.either τ1 τ2)
+| either_right
     {Γ: cx typ} {e: exp} {τ1 τ2: typ}:
     has_typ Γ e τ2 ->
-    has_typ Γ (exp.sum_right τ1 e) (typ.sum τ1 τ2)
+    has_typ Γ (exp.either_right τ1 e) (typ.either τ1 τ2)
 | case_never
     {Γ: cx typ} {e: exp} {τ: typ}:
     has_typ Γ e typ.never ->
     has_typ Γ (exp.case_never τ e) τ
 | case
     {Γ: cx typ} {eh e1 e2: exp} {x1 x2: var} {τ1 τ2 τ: typ}:
-    has_typ Γ eh (typ.sum τ1 τ2) ->
+    has_typ Γ eh (typ.either τ1 τ2) ->
     has_typ (cx.insert Γ x1 τ1) e1 τ ->
     has_typ (cx.insert Γ x2 τ2) e2 τ ->
     has_typ Γ (exp.case eh x1 e1 x2 e2) τ
