src/defs/dynamics.lean
@@ -8,9 +8,9 @@ inductive val: exp -> Prop
 | false: val exp.false
 | fn (x: var) (τ: typ) (e: exp): val (exp.fn x τ e)
 | unit: val exp.unit
-| prod {e1 e2: exp}: val e1 -> val e2 -> val (exp.prod e1 e2)
-| sum_left {τ: typ} {e: exp}: val e -> val (exp.sum_left τ e)
-| sum_right {τ: typ} {e: exp}: val e -> val (exp.sum_right τ e)
+| pair {e1 e2: exp}: val e1 -> val e2 -> val (exp.pair e1 e2)
+| either_left {τ: typ} {e: exp}: val e -> val (exp.either_left τ e)
+| either_right {τ: typ} {e: exp}: val e -> val (exp.either_right τ e)
 
 -- e ↦ e'
 inductive steps: exp -> exp -> Prop
@@ -37,39 +37,39 @@ inductive steps: exp -> exp -> Prop
     {x: var} {τ: typ} {e e2: exp} (fv_e2: fv e2 = []):
     val e2 ->
     steps (exp.app (exp.fn x τ e) e2) (subst e2 x fv_e2 e)
-| prod_e1
+| pair_e1
     {e1 e2 e1': exp}:
     steps e1 e1' ->
-    steps (exp.prod e1 e2) (exp.prod e1' e2)
-| prod_e2
+    steps (exp.pair e1 e2) (exp.pair e1' e2)
+| pair_e2
     {e1 e2 e2': exp}:
     val e1 ->
     steps e2 e2' ->
-    steps (exp.prod e1 e2) (exp.prod e1 e2')
-| prod_left_arg
+    steps (exp.pair e1 e2) (exp.pair e1 e2')
+| pair_left_arg
     {e e': exp}:
     steps e e' ->
-    steps (exp.prod_left e) (exp.prod_left e')
-| prod_left_done
+    steps (exp.pair_left e) (exp.pair_left e')
+| pair_left_done
     {e1 e2: exp}:
-    val (exp.prod e1 e2) ->
-    steps (exp.prod_left (exp.prod e1 e2)) e1
-| prod_right_arg
+    val (exp.pair e1 e2) ->
+    steps (exp.pair_left (exp.pair e1 e2)) e1
+| pair_right_arg
     {e e': exp}:
     steps e e' ->
-    steps (exp.prod_right e) (exp.prod_right e')
-| prod_right_done
+    steps (exp.pair_right e) (exp.pair_right e')
+| pair_right_done
     {e1 e2: exp}:
-    val (exp.prod e1 e2) ->
-    steps (exp.prod_right (exp.prod e1 e2)) e2
-| sum_left_arg
+    val (exp.pair e1 e2) ->
+    steps (exp.pair_right (exp.pair e1 e2)) e2
+| either_left_arg
     {τ: typ} {e e': exp}:
     steps e e' ->
-    steps (exp.sum_left τ e) (exp.sum_left τ e')
-| sum_right_arg
+    steps (exp.either_left τ e) (exp.either_left τ e')
+| either_right_arg
     {τ: typ} {e e': exp}:
     steps e e' ->
-    steps (exp.sum_right τ e) (exp.sum_right τ e')
+    steps (exp.either_right τ e) (exp.either_right τ e')
 | case_never_arg
     {τ: typ} {e e': exp}:
     steps e e' ->
@@ -80,9 +80,9 @@ inductive steps: exp -> exp -> Prop
     steps (exp.case eh x1 e1 x2 e2) (exp.case eh' x1 e1 x2 e2)
 | case_done_left
     {τ: typ} {e e1 e2: exp} {x1 x2: var} (fv_e: fv e = []):
-    val (exp.sum_left τ e) ->
-    steps (exp.case (exp.sum_left τ e) x1 e1 x2 e2) (subst e x1 fv_e e1)
+    val (exp.either_left τ e) ->
+    steps (exp.case (exp.either_left τ e) x1 e1 x2 e2) (subst e x1 fv_e e1)
 | case_done_right
     {τ: typ} {e e1 e2: exp} {x1 x2: var} (fv_e: fv e = []):
-    val (exp.sum_right τ e) ->
-    steps (exp.case (exp.sum_right τ e) x1 e1 x2 e2) (subst e x2 fv_e e2)
+    val (exp.either_right τ e) ->
+    steps (exp.case (exp.either_right τ e) x1 e1 x2 e2) (subst e x2 fv_e e2)
